>[!important] Let (R, +, $\cdot$) be a ring and let $x, y, z \in R.$ Then:
>$(i)x\cdot(y-z) = x\cdot y - x\cdot z$
> $\text{    } (y-z)\cdot x=y\cdot x-z\cdot x$
> $(ii)x\cdot 0=0\cdot x=0$
> $(iii)x\cdot(-y)=(-x)\cdot y=-x\cdot y$

**Proof:**
**(i)** We have x · (y − z) = x · y − x · z ⇐⇒ x · (y − z) + x · z = x · y ⇐⇒ x · (y − z + z) = x · y , the last equality being obviously true. Similarly, (y − z) · x = y · x − z · x. 
**(ii)** We have x · 0 = x · (y − y) = x · y − x · y = 0 . Similarly, 0 · x = 0. 
**(iii)** We have x · (−y) = −x · y ⇐⇒ x · (−y) + x · y = 0 ⇐⇒ x · (−y + y) = 0 ⇐⇒ x · 0 = 0 , the last equality being true by (ii).
$\square$
