
---
$S(V)$ - The set of all subspaces of the vector space $V$
#### Theorem 2.3.1
>[!important] Let $V$ be a vector space over $K$ and let $(S_{i})_{i\in I}$ be a family of subspaces of $V$. **Then** $\bigcap_{i\in I}S_{i}\in S(V)$

*Proof:*
For each $i\in I,\;S_{i}\in S(V)$ so $0\in S_{i}$. Then $0\in\bigcap_{i\in I}S_{i}$. Now let $k_{1}, k_{2}\in K$ and $v_{1}, v_{2}\in \bigcap_{i\in I}S_{i}$
So $v_{1}, v_{2}\in S_{i},\;\forall i\in I$. But $S_{i}\in S(V),\;\forall i\in I$. Hence, $k_{1}v_{1}+k_{2}v_{2}\in S_{i},\forall i\in I$. But this means that $k_{1}v_{1}+k_{2}v_{2}\in\bigcap_{i\in I}S_{i}$. Therefore, $\bigcap_{i\in I}S_{i}\in S(V)$ 
$\square$

#### Definition of a generator
>[!info] Let $V$ be a vector space and let $X\subseteq V$. Then we denote 
>$$\textlangle X \textrangle = \bigcap \{ S\leq V|X\subseteq S \}$$
>and we call it the *subspace generated by* $X$ or the subspace spanned by $X$. Here $X$ is called the *generating set* of $\textlangle X \textrangle$. If $X =\{ v_{1},\dots,v_{n} \}$, we denote $\textlangle v_{1},\dots,v_{n} \textrangle = \textlangle \{v_{1},\dots,v_{n}\} \textrangle$ 

#### Theorem 2.3.7
>[!important] Let $V$ be a vector space over $K$ and let $\emptyset \neq X\subseteq V$. *Then*:
>$$
>\textlangle X \textrangle = \{ k_{1}v_{1}+\dots+k_{n}v_{n}|k_{i}\in K,\;v_{i}\in X,\;i=1,\dots,n,\;n\in \mathbb{N}^{*} \}
>$$
>that is, the set of *all finite linear combinations of vectors of X*

*Proof:* We prove the result in 3 steps, by showing that 
$$L=\{ k_{1}v_{1}+\dots k_{n}v_{n}|k_{i}\in K,v_{i}\in X,i=1,\dots,n,\;n\in \mathbb{N}^{*} \}$$
is the smallest subspace of $V$ containing $X$
(i) We show that $L$ is a subspace. (ii) We show that $X\subseteq L$ (iii) We show that $L$ is the smallest subspace containing $X$
*(i)* Let $v\in X$. Then $v=1\cdot v\in L \implies L\neq \emptyset$ Now let $k,k'\in K\;and\;v,v'\in L$. 
So $v=\sum_{i=1}^nk_{i}v_{i},\;v'=\sum_{j=1}^mk_{j}v_{j}$ for some $k_{1},\dots k_{n},\;k'_{1},\dots,k'_{m}\in K$ and $v_{1},\dots,v_{n},v'_{1},\dots,v'_{n}\in X$. Then $kv+k'v'\in L$ (these two sums summed together are clearly a finite linear combination of vectors of $X$, even with a coefficient from $K$). Hence $L\leq V$
*(ii)* Let $v \in X,\;v=1\cdot v\in L \implies X\subseteq L$
*(iii)* To show that $L$ is the smallest subspace containing $X$, we take a free subspace containing $X$ and show that $L\subseteq S$, whatever subspace we are talking about, and if $L$ is included in any subspace containing $X$, then it is the smallest.
Let $S\leq V s.t\;X\subseteq S$. Let $k_{1},\dots k_{n}\in K\;and\;v_{1},\dots v_{n}\in X$. Since $X\subseteq S\;and\;S\leq V$
$$k_{1}v_{1}+\dots k_{n}v_{n}\in S\text{ (any sum of vectors of X are in S by the def. of a subspace) }$$
But this sum, which is an arbitrarily taken linear combinations of vectors of $X$, is actually L, so we have $\forall v\in L,\;v\in S$. Hence, $L\subseteq S$. So $L$ must be the smallest subspace containing $X$
**Thus**, we have $\textlangle X \textrangle = L$, by the [[#Definition of a generator]] of a set $X$, is the smallest subspace of $V$ containing $X$, which in this case is $L$.
$\square$
#### Definition of the sum of subspaces
>[!info] Let $V$ be a vector space over $K$ and let $S, T\leq V$. We define the *sum* of the subspaces $S$ and $T$ as the set
>$$S+T=\{ s+t|s \in S, t\in T \}$$

#### Theorem 2.3.11 (sum of subspaces)
>[!important] Let $V$ be a vector space over $K$ and $S, T\leq V$. Then 
>$S+T=\textlangle S\cup T \textrangle, \;hence\;S+T\leq V$.

*Proof:* We prove by the equality of the double inclusion
First, let $v=s+t\in S+T,$ for some $s \in S\;and\;t\in T$.
Then $v=1\cdot s+1\cdot t$, so $v$ is a linear combinations of vectors $s,t\in S\cup T \implies v\in \textlangle S\cup T \textrangle$
Thus, $S+T\subseteq\textlangle S\cup T \textrangle$
Now, let $v\in\textlangle S\cup T \textrangle$. Then $v=\sum_{i=1}^nv_{i}k_{i}=\sum_{i\in I}k_{i}v_{i}+\sum_{j\in J}k_{j}v_{j}$, where $I=\{ i\in \{ 1,\dots,n \}|v_{i}\in S \}$ and $J=\{ j\in \{ 1,\dots,n \}|v_{j}\in T\textbackslash S \}$
But the first sum is a linear combination of vectors from $S$, hence it $\in S$, and the second sum relating $J$ is of vectors from $T$, hence it $\in T$ (because $S$ and $T$ are subspaces). Thus, the sum of those two sums, one from $S$ and one from $T$, clearly $\in S+T$, and so $\textlangle S\cup T \textrangle \subseteq S+T$
From those two inclusions, we get $S+T=\textlangle S\cup T \textrangle$ $\square$

$\square$
#### Definition of the direct sum of subspaces
>[!info] Let $V$ be a vector space over $K$ and let $S, T\leq V$.
>If $S\cap T=\{ 0 \},\;then\;S+T$ is denoted by $S\oplus T$ and is called the *direct sum* of the subspaces $S$ and $T$>

#### Theorem 2.3.13 (Direct Sum)
>[!important] Let $V$ be a vector space over $K$ and let $S, T\leq V$. *Then*
>$$V=S\oplus T\iff \forall v\in V,\exists!s \in S, t\in T:v=s+t$$
>

*Proof:*
$\fbox{=>}$ Assume $V=S\oplus T$ . Let $v\in V$. Then $\exists s \in S,t\in T\;such\; that\;v=s+t$. 
Now suppose that $\exists s'\in S,t'\in T$ such that $v=s'+t' \implies s+t=s'+t' \implies s-s'=t-t'$.
But $s-s'\in S$ and $t-t'\in T$, and if they're equal it means they $\in S\cap T$.
But since $S+T$ is a direct sum, it means that $S\cap T=\{ 0 \}$
Thus, $s-s'=t-t'=0 \implies s=s'$ and $t=t'$, so the vectors from $S$ and $T$ that give an arbitrarily taken vector from $V$ must be unique.
$\fbox{<=}$ Assume that $\forall v\in V,\exists!s \in S,t\in T:v=s+t,$ thus $v\in S+ T$, so $V\subseteq S+T$
Clearly, we also have, since $S+T$ is a subspace $S+T\subseteq V$. Thus, $S+T=V$ 
Now, to prove that $S\cap T=\{ 0 \}$, assume that $\exists v\neq 0\in S\cap T$. Then $v=v+0=0+v\in S+T$. But this is a contradiction, since we have the uniqueness of writing $v$ as a sum of an element from $S$ and an element from $T$, and in this case , we can write it in TWO ways: take $v$ from $S$ and $0$ from $T$ , or vice-versa, and $0\neq v$, so $s\neq s'$. 
Therefore, $S\cap T=\{ 0 \}$, and by [[#Definition of the direct sum of subspaces]], $V=S\oplus T$
$\square$

---


